overloaded reading and writing for pointers and buffers

ulib/LowStar.Lens.Buffer.fst
@@ -25,77 +25,187 @@ open FStar.Integers
    buffers, allowing viewing a hyperstack containing a buffer as just
    a sequence of the buffer's contents.
    
-   This is one of two main "leaf" instance of an `hs_lens`, since
-   (almost) all mutable types in LowStar are expressed via monotonic
-   buffers.
+   This is the main "leaf" instance of an `hs_lens`, since (almost)
+   all mutable types in LowStar are expressed via monotonic buffers
+   (referring to a sequence) or pointers (referring to a single
+   element).
 
-   The other one is LowStar.Lens.Pointer
+   This module multiplexes between the buffer and pointer views as "two
+   flavors".
 
-   The `ref` types are an exception: for convenient use with LensST,
-   we recommend using `pointer` instead of `ref`.
-*)
+   Note, Low* also supports `ref` types, which are essentially
+   equivalent to pointers. For uniformity, we recommend using `pointer`
+   instead of `ref`.  *)
+
+/// `flav`: Two varieties of references
+type flav =
+  | Buffer
+  | Pointer
+
+/// `ok_for_ptr q`: Pointers, unfortunately, are indexed by preorders on
+/// sequences, rather than preorders on elements. So, we need some
+/// conditions to ensure that a sequence preorder is appropriate for a
+/// pointer.
+let ok_for_ptr (q:B.srel 'a) =
+  forall (s0 s1 : Seq.seq 'a). {:pattern (s0 `q` s1)}
+    (Seq.length s0 == Seq.length s1 /\
+     Seq.length s0 == 1 /\
+     (Seq.create 1 (Seq.index s0 0)) `q` (Seq.create 1 (Seq.index s1 0))) ==>
+    s0 `q` s1
+
+/// `flavor`: A buffer `b` is described as Pointer-flavor if
+///  -- its length is 1
+///  -- its preorder is ok for pointers
+let flavor #a #p #q (b:B.mbuffer a p q) =
+  f:flav{ 
+    f == Pointer ==>
+    B.length b == 1 /\
+    ok_for_ptr q
+  }
+
+
+/// A couple of convenient flavor abbreviations
+unfold 
+let ptr (b:B.pointer 'a) : flavor b = Pointer
+
+unfold 
+let buf (b:B.mbuffer 'a 'b 'c) : flavor b = Buffer
+
 
 /// `lseq_of`: A sequence whose length matches the buffer's length
 let lseq_of #a #p #q (b:B.mbuffer a p q) =
   Seq.lseq a (B.length b)
 
+/// `view_type_of b f`: Provides an f-flavored voew on the buffer `b`
+let view_type_of #a #p #q (b:B.mbuffer a p q) (f:flavor b) =
+  match f with
+  | Buffer -> lseq_of b
+  | Pointer -> a
+
 /// `buffer_hs_lens`:
 ///   hs_lens between a buffer `b` and `lseq_of b`
-let buffer_hs_lens #a #p #q (b:B.mbuffer a p q) =
-  l:hs_lens (B.mbuffer a p q) (lseq_of b){
+///   of flavor `f`
+let buffer_hs_lens #a #p #q (b:B.mbuffer a p q) (f:flavor b) =
+  l:hs_lens (B.mbuffer a p q) (view_type_of b f){
     Ghost.reveal l.footprint == B.loc_buffer b
   }
 
-/// `reader_t l`: reads a single element out of a buffer
-let reader_t #a #p #q (#b:B.mbuffer a p q) (lens:buffer_hs_lens b) =
-  i:uint_32{ i < B.len b } ->
-  with_state lens a
-    (requires fun _ -> True)
-    (ensures fun s0 v s1 ->
-      s0 == s1 /\
-      v == Seq.index s1 (UInt32.v i))
+/// `get_value_at` and `put_value_at`: provide a uniform sequence- or
+///  element-based view on top of both flavors of buffers
+unfold
+let get_value_at #a #p #q (#b:B.mbuffer a p q) (#f:flavor b)
+                 (v:view_type_of b f)
+                 (i:uint_32{ i < B.len b })
+    : a =
+    match f with
+    | Pointer -> v
+    | Buffer -> Seq.index v (UInt32.v i)
 
-/// `reader_t l`: writes a single element to a buffer
-let writer_t #a #p #q (#b:B.mbuffer a p q) (lens:buffer_hs_lens b) =
-  i:uint_32{ i < B.len b } ->
-  v:a ->
-  with_state lens unit
-    (requires fun s0 -> 
-      s0 `q` Seq.upd s0 (UInt32.v i) v)
-    (ensures fun s0 _ s1 ->
-      s1 `Seq.equal` Seq.upd s1 (UInt32.v i) v)
+unfold
+let put_value_at #a #p #q (#b:B.mbuffer a p q) (#f:flavor b)
+                 (v0:view_type_of b f)
+                 (i:uint_32{ i < B.len b })
+                 (x:a)
+    : view_type_of b f =
+    match f with
+    | Pointer -> x
+    | Buffer -> Seq.upd v0 (UInt32.v i) x
+
+/// `as_seq` views both flavors as a sequence
+unfold
+let as_seq #a #p #q 
+           (#b:B.mbuffer a p q)
+           (#f:flavor b)
+           (v0:view_type_of b f)
+   : lseq_of b
+   = match f with
+     | Pointer -> Seq.create 1 v0
+     | Buffer -> v0
+
+
+/// `with_state t`:
+///
+///    A computation in `LensST` which supports updating the snapshot
+///
+///    This is a technical device, not intended for typical use in
+///    client code, but is useful in libraries that provide support for
+///    composing and de-composing hs_lenses.
+let with_state #from #to
+               (lens:hs_lens from to)
+               ($t:hs_lens from to -> Type) =
+  s:imem (lens.invariant lens.x) ->
+  t (snap lens s)
+
+let ix #a #p #q (b:B.mbuffer a p q) = i:uint_32{i < B.len b}
+
+module LL = LowStar.Lens
+/// `writer_t l`: writes a single element to a buffer
+let reader_t #a #p #q (#b:B.mbuffer a p q) (f:flavor b)
+             #from #to (layer: lens to (view_type_of b f))
+             (l:hs_lens from to)
+  = i:ix b ->
+    LensST a l
+      (requires fun _ -> True)
+      (ensures fun s0 v s1 ->
+        s0 == s1 /\
+        v == get_value_at (LL.get layer s1) i)
+
+/// `writer_t l`: writes a single element to a buffer
+let writer_t #a #p #q (#b:B.mbuffer a p q) (f:flavor b)
+             #from #to (layer: lens to (view_type_of b f))
+             (l:hs_lens from to)
+  = i:ix b ->
+    v:a ->
+    LensST unit l
+      (requires fun s0 ->
+        as_seq (LL.get layer s0) `q` as_seq (put_value_at (LL.get layer s0) i v))
+      (ensures fun s0 _ s1 ->
+        s1 == LL.put layer s0 (put_value_at (LL.get layer s0) i v))
+
+unfold
+let id_lens #a : lens a a = {
+  get= (fun x -> x);
+  put= (fun x s -> x);
+  lens_laws = ()
+}
 
 /// `buffer_lens`: A triple of a lens for a buffer and its
 /// corresponding element readers and writers
 noeq
-type buffer_lens #a #p #q (b:B.mbuffer a p q) =
-  | Mk : hs_lens:buffer_hs_lens b ->
-         reader:reader_t hs_lens ->
-         writer:writer_t hs_lens ->
-         buffer_lens b
+type buffer_lens #a #p #q (b:B.mbuffer a p q) (f:flavor b) =
+  | Mk : hs_lens:buffer_hs_lens b f ->
+         reader:with_state hs_lens (reader_t f id_lens) ->
+         writer:with_state hs_lens (writer_t f id_lens)  ->
+         buffer_lens b f
 
 /// `lens_of`: Projecting out the `hs_lens` from a `buffer_lens`
-let lens_of #a #p #q (#b:B.mbuffer a p q) (prw:buffer_lens b)
-   : buffer_hs_lens b
+let lens_of #a #p #q (#b:B.mbuffer a p q) (#f:flavor b) (prw:buffer_lens b f)
+   : buffer_hs_lens b f
    = prw.hs_lens
 
 /// `mk`: Constructs a buffer_lens from a buffer and a given state
 abstract
-let mk #a #p #q (b:B.mbuffer a p q) (snap:HS.mem{B.live snap b})
-  : Tot (l:buffer_lens b{(lens_of l).snapshot == snap})
-  = let blens : buffer_hs_lens b =
+let mk #a #p #q (b:B.mbuffer a p q) (f:flavor b) (snap:HS.mem{B.live snap b})
+  : Tot (l:buffer_lens b f{(lens_of l).snapshot == snap})
+  = let blens : buffer_hs_lens b f =
         FStar.Classical.forall_intro_2 (B.g_upd_seq_as_seq b);
         let invariant (x:B.mbuffer a p q) (h:HS.mem) =
           B.live h x
         in
         let fp = Ghost.hide (B.loc_buffer b) in
-        let get : get_t (imem (invariant b)) (lseq_of b) =
-          fun h -> B.as_seq h b
+        let get : get_t (imem (invariant b)) (view_type_of b f) =
+          fun h -> 
+            match f with
+            | Buffer -> B.as_seq h b
+            | Pointer -> B.get h b 0
         in
-        let put : put_t (imem (invariant b)) (lseq_of b) =
-          fun v h -> B.g_upd_seq b v h
+        let put : put_t (imem (invariant b)) (view_type_of b f) =
+          fun v h ->
+            match f with
+            | Buffer -> B.g_upd_seq b v h
+            | Pointer -> B.g_upd b 0 v h
         in
-        let l : imem_lens (invariant b) (lseq_of b) fp = {
+        let l : imem_lens (invariant b) (view_type_of b f) fp = {
           get = get;
           put = put;
           lens_laws = ()
@@ -109,13 +219,13 @@ let mk #a #p #q (b:B.mbuffer a p q) (snap:HS.mem{B.live snap b})
           l = l
         }
     in
-    let reader : reader_t blens =
-      fun i s ->
+    let reader : with_state blens (reader_t f id_lens) =
+      fun s i ->
         reveal_inv();
         B.index b i
     in
-    let writer : writer_t blens =
-      fun i v s ->
+    let writer : with_state blens (writer_t f id_lens) =
+      fun s i v ->
         reveal_inv();
         B.upd b i v
     in
@@ -124,40 +234,36 @@ let mk #a #p #q (b:B.mbuffer a p q) (snap:HS.mem{B.live snap b})
 /// `elim_inv`: Revealing the abstract invariant of buffer lenses
 let elim_inv #a #p #q 
              (#b:B.mbuffer a p q)
-             (bl:buffer_lens b)
+             (#f:flavor b)
+             (bl:buffer_lens b f)
              (h:HS.mem)
   : Lemma (let l = lens_of bl in
-           (exists h'.{:pattern mk b h'} B.live h' b /\ bl == mk b h') /\
+           (exists h'.{:pattern mk b f h'} B.live h' b /\ bl == mk b f h') /\
             inv l h ==>
              B.live h b /\
-             view l h == B.as_seq h b)
+             view l h == (match f with
+                          | Pointer -> B.get h b 0
+                          | Buffer -> B.as_seq h b))
   = reveal_inv ()
 
 /// `index`: The analog of LowStar.Monotonic.Buffer.index
 let index #a #p #q 
           (#b:B.mbuffer a p q)
-          (bl:buffer_lens b)
-          (i:uint_32{i < B.len b})
-  : LensST a (lens_of bl)
-    (requires fun _ -> True)
-    (ensures fun s0 v s1 ->
-      s0 == s1 /\
-      v == Seq.index s1 (UInt32.v i))
-  = reveal_inv ();
+          (#f:flavor b)
+          (bl:buffer_lens b f)
+  : reader_t f id_lens (lens_of bl)
+  = fun i -> 
+    reveal_inv ();
     let h = HST.get() in
-    bl.reader i h
+    bl.reader h i
 
 /// `upd`: The analog of LowStar.Monotonic.Buffer.upd
 let upd #a #p #q 
           (#b:B.mbuffer a p q)
-          (bl:buffer_lens b)
-          (i:uint_32{i < B.len b})
-          (v:a)
-  : LensST unit (lens_of bl)
-    (requires fun s0 ->
-      s0 `q` Seq.upd s0 (UInt32.v i) v)
-    (ensures fun s0 _ s1 ->
-      s1 `Seq.equal` Seq.upd s1 (UInt32.v i) v)
-  = reveal_inv ();
+          (#f:flavor b)
+          (bl:buffer_lens b f)
+  : writer_t f id_lens (lens_of bl)
+  = fun i v -> 
+    reveal_inv ();
     let h = HST.get() in
-    bl.writer i v h
+    bl.writer h i v
